

Supplementary Calculus Notes

Econ 3020 - Winter 2026

Tie Ma

January 6, 2026

Disclaimer

Important Note

This document is intended as a **supplement** to, not a substitute for, the official lectures

- This is **unofficial reference material**. Please always refer to the Professor's lectures and slides for definitive course content and notation.
- **Rule of Thumb:** In the event of any discrepancy between these notes and the Professor's materials, **the Professor's materials take precedence**.

1 Basic Derivatives

Consider the function where $x \in \mathbb{R}$:

$$f(x) = x^2 \tag{1}$$

First Derivative (f')

Using the Power Rule:

$$\begin{aligned}\frac{df}{dx} &= 2x^{2-1} \\ \frac{df}{dx} &= 2x^1 \\ \frac{df}{dx} &= 2x\end{aligned}$$

Or simply: $f'(x) = 2x$.

Second Derivative (f'')

We differentiate the first derivative with respect to x :

$$\begin{aligned}\frac{d}{dx} \left(\frac{df}{dx} \right) &= \frac{d}{dx}(2x) \\ &= (2)(1)x^{1-1} \\ \frac{d^2f}{dx^2} &= 2x^0 \\ \frac{d^2f}{dx^2} &= 2\end{aligned}$$

Third Derivative (f''')

We differentiate the second derivative with respect to x :

$$\begin{aligned}\frac{d}{dx} \left(\frac{d^2f}{dx^2} \right) &= \frac{d}{dx}(2) \\ \frac{d^3f}{dx^3} &= 0\end{aligned}$$

(The derivative of a constant is always 0).

Example 2: Constant Multiples

Consider the function where $x \in \mathbb{R}$:

$$f(x) = 2x^2 \tag{2}$$

Derivatives:

$$\begin{aligned}\frac{df}{dx} &= 4x \\ \frac{d^2f}{dx^2} &= 4 \\ \frac{d^3f}{dx^3} &= 0\end{aligned}$$

Example 3: Additive Rule

Consider the function where $x \in \mathbb{R}$:

$$f(x) = 2x^2 + x^3 \tag{3}$$

Apply the power rule to each term separately:

$$\begin{aligned}f'(x) &= 2 \cdot (2x^{2-1}) + 3x^{3-1} \\ f'(x) &= 4x^1 + 3x^2\end{aligned}$$

Example 4: Constants

Consider the function below.

The derivative of a constant is 0 because it does not change.

$$f(x) = x^2 + 3 \tag{4}$$

$$\begin{aligned}\frac{df}{dx} &= \frac{d}{dx}(x^2) + \frac{d}{dx}(3) \\ \frac{df}{dx} &= 2x^{2-1} + 0 \\ \frac{df}{dx} &= 2x\end{aligned}$$

Example 5: Chain Rule

Consider the function:

$$f(x) = (x^2 + 3)^3 \tag{5}$$

The rule is: *differentiate the outside first, then the inside.*

$$\begin{aligned}f'(x) &= 3(x^2 + 3)^{3-1} \cdot \frac{d}{dx}(x^2 + 3) \\f'(x) &= 3(x^2 + 3)^2 \cdot (2x) \\f'(x) &= 6x(x^2 + 3)^2\end{aligned}$$

Addition Note

It is helpful to distinguish between the **result** and the **operation**:

- $\frac{df}{dx}$ (**The Result**): This symbol represents the derivative of the function f . It is a noun. It refers to the final answer.
- $\frac{d}{dx}$ (**The Operator**): This symbol is an instruction or command. It represents the **action** of taking the derivative with respect to x . It tells you to differentiate whatever comes immediately after it.

Example:

$$\frac{d}{dx}(x^2) = 2x \tag{6}$$

In this equation:

- $\frac{d}{dx}$ is the instruction: "Differentiate x^2 ".
- $2x$ is the result ($\frac{df}{dx}$).

Example 6: Product Rule

Let $x \in \mathbb{R}_{++}$.

The rule is **Derivative of the first times the second, PLUS derivative of the second times the first.**

$$(uv)' = u'v + uv'$$

First Derivative (f')

Using the Product Rule:

$$\begin{aligned}f(x) &= x^2(x^2 + 3)^3 \\f'(x) &= \frac{d}{dx}(x^2) \cdot (x^2 + 3)^3 + x^2 \cdot \frac{d}{dx}((x^2 + 3)^3) \\&= 2x(x^2 + 3)^3 + x^2 \cdot 3(x^2 + 3)^2 \cdot (2x) \\&= 2x(x^2 + 3)^3 + 6x^3(x^2 + 3)^2 \\&= 2x(x^2 + 3)^2 [(x^2 + 3) + 3x^2] \\&= 2x(x^2 + 3)^2(4x^2 + 3)\end{aligned}$$

Example 7: Negative Exponents

Let $x \in \mathbb{R}_{++}$.

- \mathbb{R}_{++} means strictly positive numbers (excluding 0).
- \mathbb{R}_+ means positive numbers (including 0).

Consider:

$$f(x) = \frac{1}{x} = x^{-1} \tag{7}$$

Apply the power rule:

$$\begin{aligned}f'(x) &= -1 \cdot x^{-1-1} \\f'(x) &= -1 \cdot x^{-2} \\f'(x) &= -\frac{1}{x^2}\end{aligned}$$

Practice Question

Find $\frac{df}{dx}$ for:

$$f(x) = \frac{1}{(x^2 + 3)^3} = (x^2 + 3)^{-3} \tag{8}$$

Solution:

$$\begin{aligned}f'(x) &= (-3)(x^2 + 3)^{-3-1} \cdot \frac{d}{dx}(x^2 + 3) \\f'(x) &= (-3)(x^2 + 3)^{-4} \cdot (2x) \\f'(x) &= -6x(x^2 + 3)^{-4}\end{aligned}$$

To write this as a fraction, the negative exponent moves to the denominator and becomes positive:

$$f'(x) = \frac{-6x}{(x^2 + 3)^4} \quad (9)$$

Example 8: Quotient Rule

Let $x \in \mathbb{R}_{++}$.

$$f(x) = \frac{x^2}{2x + 1} \quad (10)$$

The Quotient Rule is: "Low d-High minus High d-Low, over Low squared":

$$\left(\frac{u}{v}\right)' = \frac{u'v - uv'}{v^2}$$

Applying the rule:

$$\begin{aligned} f'(x) &= \frac{(2x)(2x + 1) - (x^2)(2)}{(2x + 1)^2} \\ &= \frac{4x^2 + 2x - 2x^2}{(2x + 1)^2} \\ &= \frac{2x^2 + 2x}{(2x + 1)^2} \end{aligned}$$

2 Two Variables and Partial Derivatives

Example 9: Cobb-Douglas Function

Consider a standard Cobb-Douglas function (Multiplicative):

$$f(x, y) = x^\alpha y^\beta \quad (11)$$

Find $\frac{\partial f}{\partial x}$: We treat y as a constant.

$$\frac{\partial f}{\partial x} = \alpha x^{\alpha-1} \cdot y^\beta$$

Example 10: Additive Function

Consider the function where $x, y \in \mathbb{R}$:

$$f(x, y) = x^2 + y^2 \quad (12)$$

Find $\frac{\partial f}{\partial x}$: We treat y as a constant. Since y is constant, y^2 is also a constant, so its derivative is 0.

$$\begin{aligned} \frac{\partial f}{\partial x} &= \frac{\partial}{\partial x}(x^2) + \frac{\partial}{\partial x}(y^2) \\ \frac{\partial f}{\partial x} &= 2x + 0 \\ \frac{\partial f}{\partial x} &= 2x \end{aligned}$$

The rest part is the same, so I will not cover.

Example 11: Exponents and Logs

Let $x \in \mathbb{R}_{++}$ (so that $\ln(x)$ is defined).

$$f(x) = e^x \quad (13)$$

find $f'(x)$

$$\frac{d}{dx}(a^x) = a^x \cdot \ln(a) \quad (14)$$

then

$$\frac{d}{dx}(e^x) = e^x \cdot \ln(e) \quad (15)$$

$$\frac{d}{dx}(e^x) = e^x \cdot 1 \quad (16)$$

for the e the difference thing we will use the chain rule

$$f(x) = e^{3x} \quad (17)$$

$$\frac{d}{dx}(e^{3x}) = e^{3x} \cdot \frac{d}{dx}3x \text{ (chain rule)} \quad (18)$$

$$\frac{d}{dx}(e^{3x}) = e^{3x} \cdot 3 \quad (19)$$

$$\frac{d}{dx}(e^{3x}) = 3e^{3x} \quad (20)$$

$$f(x) = \ln(x) \quad \Rightarrow \quad f'(x) = \frac{1}{x} \quad (21)$$

$$f'(x) = \frac{1}{x} \quad (22)$$

$$f(x) = \ln(x^2) \quad (23)$$

Method 1

$$\begin{aligned} f'(x) &= \frac{1}{x^2} \cdot 2x \\ &= f'(x) = \frac{2}{x} \end{aligned}$$

Method 2

$$\begin{aligned} f(x) &= \ln(x^2) \\ &= f(x) = 2 \cdot \ln(x) \\ &= f'(x) = 2 \cdot \frac{1}{x} \\ &= f'(x) = \frac{2}{x} \end{aligned}$$

Consider the function:

$$f(x) = \ln [(x^3 + 4)^2] \quad (24)$$

find $f'(x)$

Method 1

$$\begin{aligned}f'(x) &= \frac{1}{(x^3 + 4)^2} \cdot \frac{d}{dx}((x^3 + 4)^2) \\&= \frac{1}{(x^3 + 4)^2} \cdot [2(x^3 + 4)^1 \cdot 3x^2] \\&= \frac{6x^2(x^3 + 4)}{(x^3 + 4)^2} \\&= \frac{6x^2}{x^3 + 4}\end{aligned}$$

Method 2

First, bring the exponent down using the rule $\ln(a^b) = b \ln a$:

$$f(x) = 2 \ln(x^3 + 4) \tag{25}$$

$$\begin{aligned}f'(x) &= 2 \cdot \frac{d}{dx}(\ln(x^3 + 4)) \\&= 2 \cdot \frac{1}{x^3 + 4} \cdot (3x^2) \\&= \frac{6x^2}{x^3 + 4}\end{aligned}$$

Example 12: Total Differential

Mathematical Assumption

For the Total Differential to exist and for the linear approximation to work, we assume the function $f(x, y)$ is "**Smooth**". Mathematically, this means:

1. **Continuity:** The function has no holes or jumps.
2. **Continuous Partial Derivatives:** The rate of change does not jump suddenly. The surface has no sharp corners or kinks.

Now, let's start with the Cobb-Douglas utility function:

$$U(x, y) = x^{1-a}y^a \tag{26}$$

where $a \in (0, 1)$.

The formula for the **Total Differential** is:

$$dU = \frac{\partial U}{\partial x} dx + \frac{\partial U}{\partial y} dy \quad (27)$$

Step 1: Find the Marginal Utility of x ($\frac{\partial U}{\partial x}$) Treat y as a constant.
Apply the Power Rule to x^{1-a} :

$$\begin{aligned} \frac{\partial U}{\partial x} &= (1-a)x^{(1-a)-1} \cdot y^a \\ &= (1-a)x^{-a}y^a \end{aligned}$$

This represents the rate at which utility increases as we add more of good x , holding good y constant.

Step 2: Find the Marginal Utility of y ($\frac{\partial U}{\partial y}$) Treat x as a constant.
Apply the Power Rule to y^a :

$$\begin{aligned} \frac{\partial U}{\partial y} &= x^{1-a} \cdot ay^{a-1} \\ &= ax^{1-a}y^{a-1} \end{aligned}$$

Similarly, this is the rate of utility change from an increase in good y , holding good x constant.

Step 3: Combine into the Total Differential

$$dU = [(1-a)x^{-a}y^a] dx + [ax^{1-a}y^{a-1}] dy \quad (28)$$

This equation sums up the effects. It tells us the total change in utility when the quantities of both x and y change at the same time.

Indifference Curve and MRS

By the definition of an indifference curve, the consumer is **indifferent** between bundles along the curve. Mathematically, this implies utility is constant, so $dU = 0$.

$$0 = MU_x dx + MU_y dy \quad (29)$$

Rearranging terms to put dx and dy on opposite sides:

$$-MU_y dy = MU_x dx \quad (30)$$

To find the slope of the indifference curve ($\frac{dy}{dx}$), we divide both sides by dx and MU_y :

$$\frac{dy}{dx} = -\frac{MU_x}{MU_y} \quad (31)$$

Assumption: Strict Monotonicity

Theoretically, the axiom of **Local Non-Satiation (LNS)** ensures there is always a direction to make the consumer better off. However, for simplicity, we assume **Strict Monotonicity** ("More is Better").

This ensures:

1. Marginal Utilities are strictly positive: $MU_x > 0$ and $MU_y > 0$.
2. The solution lies **on** the budget line.

Marginal Rate of Substitution (MRS)

The **Marginal Rate of Substitution** is defined as the absolute value of the slope of the indifference curve:

$$MRS_{xy} = \left| \frac{dy}{dx} \right| = \frac{MU_x}{MU_y} \quad (32)$$

Optimization will be covered in the file `addition_calculus.2`. (If you cannot find it, I probably haven't finished it yet).

Postscript

I have always wanted to write a set of supplementary notes, both to review the math content for myself and to provide extra help for students who need it. However, I could never seem to find the opportunity to sit down and start writing.

The first draft of these notes was finally finished on a train during my 2025 Winter Break. Thanks to the poor internet connection on board, I was able to disconnect and focus entirely on this work.